src/ShouldBuild.v
@@ -1,4 +1,5 @@
 From Perennial Require Import program_logic.crash_lang.
+From Perennial Require Import program_logic.crash_weakestpre.
 
 
 (* examples on top of concurrency framework *)
